store/client_proofs/close.v
@@ -36,24 +36,21 @@ Lemma wp_client_close c kI kR cs :
 Proof.
 iIntros "#chan_c (_ & _ & _ & _ & _ & _ & _ & _ & #close & #ack & _)".
 iIntros "!> %Φ client post".
-iDestruct "client" as "(%n & %beginning & <- & <- & conn & client)".
+iDestruct "client" as "(%n & %beginning & <- & <- & #conn & ts & client)".
 wp_lam; wp_pures.
-wp_bind (Connection.timestamp _).
-iApply (wp_connection_timestamp with "conn").
-iIntros "!> conn". wp_pures.
-wp_bind (tint _). iApply wp_tint. wp_pures.
+wp_apply (wp_connection_timestamp with "ts"). iIntros "ts".
+wp_pures. wp_apply wp_tint. wp_pures.
 iMod (close_predI with "client") as "(client & #p_m1)" => //.
 wp_bind (Connection.send _ _ _ _).
-iApply (wp_connection_send with "[//] close [] [//] conn") => //.
+wp_apply (wp_connection_send with "[//] close [] [//] conn") => //.
 { by rewrite public_TInt. }
-iIntros "!> conn". wp_pures.
-iCombine "client post" as "I". iRevert "conn I".
+iIntros "_". wp_pures.
+iCombine "client post" as "I". iRevert "ts I".
 iApply wp_connection_recv => //.
-iIntros "!> %m conn (client & post) #m_m #inv'".
+iIntros "!> %m ts (client & post) #m_m #inv'".
 iMod (ack_close_predE with "client inv'") as "client" => //.
-wp_pures. wp_bind (Connection.close _ _).
-iApply (wp_connection_close with "conn"). iIntros "!> _".
-wp_pures.
+wp_pures. wp_apply (wp_connection_close with "ts").
+iIntros "_". wp_pures.
 iRight. iModIntro. iExists _. iSplit; eauto.
 iApply "post".
 iExists _. by eauto.
