store/connection_proofs.v
@@ -32,7 +32,8 @@ Lemma wp_connection_connect N c kI kR :
   {{{ True }}}
     Connection.connect N c kI (TKey Open kR)
   {{{ cs, RET (repr cs);
-    is_conn_state cs 0 ∗
+    wf_conn_state cs ∗
+    cs_ts cs ↦ #0 ∗
     ⌜si_init cs = kI⌝ ∗
     ⌜si_resp cs = kR⌝ ∗
     ⌜cs_role cs = Init⌝ ∗
@@ -64,7 +65,8 @@ Lemma wp_connection_listen N c kR :
   {{{ True }}}
     Connection.listen N c kR
   {{{ cs, RET (TKey Open (si_init cs), repr cs)%V;
-    is_conn_state cs 0 ∗
+    wf_conn_state cs ∗
+    cs_ts cs ↦ #0 ∗
     ⌜si_resp cs = kR⌝ ∗
     ⌜cs_role cs = Resp⌝ ∗
     term_token (si_resp_share cs) ⊤ }}}.
@@ -88,56 +90,52 @@ rewrite /failure. by eauto.
 Qed.
 
 Lemma wp_connection_timestamp cs (n : nat) :
-  {{{ is_conn_state cs n }}}
+  {{{ cs_ts cs ↦ #n }}}
     Connection.timestamp (repr cs)
-  {{{ RET #n; is_conn_state cs n }}}.
+  {{{ RET #n; cs_ts cs ↦ #n }}}.
 Proof.
 rewrite /Connection.timestamp.
-iIntros "%Φ (Hn & #? & #key) post".
-wp_pures. wp_load. iApply "post". iModIntro. iFrame. by eauto.
+iIntros "%Φ Hn post".
+wp_pures. wp_load. iApply "post". iModIntro. by iFrame.
 Qed.
 
 Lemma wp_connection_tick cs (n : nat) :
-  {{{ is_conn_state cs n }}}
+  {{{ cs_ts cs ↦ #n }}}
     Connection.tick (repr cs)
-  {{{ RET #(); is_conn_state cs (S n) }}}.
+  {{{ RET #(); cs_ts cs ↦ #(S n) }}}.
 Proof.
-iIntros "%Ψ (Hn & #? & #key) post".
+iIntros "%Ψ Hn post".
 rewrite /Connection.tick; wp_pures; wp_load; wp_store.
 iApply "post".
 rewrite (_ : (n + 1)%Z = (S n)%nat :> Z); last by lia.
 iFrame; eauto.
 Qed.
 
-Lemma wp_connection_session_key cs n :
-  {{{ is_conn_state cs n }}}
+Lemma wp_connection_session_key cs :
+  {{{ True }}}
     Connection.session_key (repr cs)
-  {{{ RET (repr (si_key cs));
-      is_conn_state cs n ∗
-      minted (si_key cs) ∗
-      □ (∀ kt, public (TKey kt (si_key cs)) ↔ ◇ public (si_key cs)) ∗
-      (failure (si_init cs) (si_resp cs) ∨
-       □ (◇ public (si_key cs) ↔ ▷ False)) }}}.
+  {{{ RET (repr (si_key cs)); True }}}.
 Proof.
 rewrite /Connection.session_key.
-iIntros "%Φ (? & #? & #? & #?) post". wp_pures. iApply "post".
-iModIntro. iFrame. iSplit => //; eauto.
+iIntros "%Φ _ post". wp_pures. iApply "post".
+iModIntro. by iFrame.
 Qed.
 
-Lemma wp_connection_send N c cs n m φ :
+Lemma wp_connection_send N c cs m φ :
   channel c -∗
   seal_pred N (session_msg_pred φ) -∗
   public m -∗
   failure (si_init cs) (si_resp cs) ∨ □ φ cs m -∗
-  {{{ is_conn_state cs n }}}
+  wf_conn_state cs -∗
+  {{{ True }}}
     Connection.send N c (repr cs) m
-  {{{ RET #(); is_conn_state cs n }}}.
+  {{{ RET #(); True }}}.
 Proof.
-iIntros "#chan #pred #public_m #inv !> %Φ conn post".
+iIntros "#chan #pred #public_m #inv #conn !> %Φ _ post".
+iDestruct "conn" as "(? & #? & ?)".
 wp_lam. wp_pures.
-wp_bind (Connection.session_key _).
-iApply (wp_connection_session_key with "conn").
-iIntros "!> (conn & #sess & #minted_k & #sec)". wp_pures.
+wp_apply (wp_connection_session_key _) => //.
+iIntros "_". wp_pures.
 wp_apply wp_senc. wp_pures.
 iApply wp_send => //.
 { iApply public_TSealIS => //.
@@ -256,38 +254,40 @@ Definition handler_correct φ Φ cs handler n : iProp :=
     ∃ Ψ, seal_pred handler.1 (session_msg_pred Ψ) ∗
     □ ∀ m, ▷ public m -∗
            □ ▷ (failure (si_init cs) (si_resp cs) ∨ Ψ cs m) -∗
-           is_conn_state cs n -∗
+           wf_conn_state cs -∗
+           cs_ts cs ↦ #n -∗
            φ -∗
            WP (f : val) m {{ v,
-             ⌜v = NONEV⌝ ∗ is_conn_state cs n ∗ φ ∨
+             ⌜v = NONEV⌝ ∗ cs_ts cs ↦ #n ∗ φ ∨
              ∃ r, ⌜v = SOMEV r⌝ ∗ Φ r }}
   }}%I.
 
 Lemma wp_connection_select φ Φ (c : val) cs n (handlers : list (namespace * expr)) :
   channel c -∗
   ([∗ list] handler ∈ handlers, handler_correct φ Φ cs handler n) -∗
-  is_conn_state cs n -∗
+  wf_conn_state cs -∗
+  cs_ts cs ↦ #n -∗
   φ -∗
   WP Connection.select c (repr cs) handlers {{ Φ }}.
 Proof.
 rewrite Connection.select_eq /Connection.select_def.
-iIntros "#chan_c wps conn inv".
+iIntros "#chan_c wps #conn ts inv".
 wp_bind (Connection.make_handlers _).
 iApply (wp_wand with "[wps]").
 { iApply (wp_connection_make_handlers
-            (is_conn_state cs n ∗ φ) Φ (si_key cs)
+            (cs_ts cs ↦ #n ∗ φ) Φ (si_key cs)
            with "[wps]").
   iApply (big_sepL_impl with "wps").
   iIntros "!> % %handler _ wp".
   iApply (wp_wand with "wp").
-  iIntros "%f #wp !> %m #p_m [conn inv]".
+  iIntros "%f #wp !> %m #p_m [ts inv]".
   iDestruct "wp" as "(%Ψ & #seal & #wp)".
   iAssert (minted m) as "#m_m".
   { rewrite public_minted minted_TSeal minted_tag.
     by iDestruct "p_m" as "[??]". }
   iAssert (□ ▷ (public m ∗ (failure (si_init cs) (si_resp cs) ∨ Ψ cs m)))%I
     as "{p_m} #[p_m inv_m]".
-  { iDestruct "conn" as "(? & #? & #s_key & #sess)".
+  { iDestruct "conn" as "(#? & #s_key & #sess)".
     iDestruct (public_TSealE with "[//] [//]") as "{p_m} [[p_key p_m]|p_m]".
     - iSplitR => //.
       iDestruct "sess" as "[fail|#s_key']"; first by eauto.
@@ -297,13 +297,10 @@ iApply (wp_wand with "[wps]").
       iModIntro. iModIntro.
       iDestruct "p_m" as "(%si & %e_kS & #sess' & inv_m)".
       rewrite (session_agree e_kS). by iSplit. }
-  iApply ("wp" with "p_m [//] conn inv"). }
+  iApply ("wp" with "p_m [//] conn ts inv"). }
 iIntros "% (%handlers' & -> & #Hhandlers')".
-wp_pures.
-wp_bind (Connection.session_key _).
-iApply (wp_connection_session_key with "conn").
-iIntros "!> (conn & #m_kS & #p_kS & #sess)".
-wp_pures. iCombine "conn inv" as "I". iRevert "I". iApply wp_do_until.
+wp_pures. wp_apply wp_connection_session_key => //. iIntros "_".
+wp_pures. iCombine "ts inv" as "I". iRevert "I". iApply wp_do_until.
 iIntros "!> I". wp_pures. wp_bind (recv _). iApply wp_recv => //.
 iIntros "%m #p_m". wp_pures.
 wp_apply wp_key.
@@ -321,25 +318,25 @@ Qed.
 Lemma wp_connection_recv N c cs n (f : val) φ Φ Ψ :
   channel c -∗
   seal_pred N (session_msg_pred Φ) -∗
+  wf_conn_state cs -∗
   □ (∀ m,
-      is_conn_state cs n -∗
+      cs_ts cs ↦ #n -∗
       φ -∗
       public m -∗
       □ (failure (si_init cs) (si_resp cs) ∨ Φ cs m) -∗
-      WP f m {{ v, ⌜v = NONEV⌝ ∗ is_conn_state cs n ∗ φ ∨
+      WP f m {{ v, ⌜v = NONEV⌝ ∗ cs_ts cs ↦ #n ∗ φ ∨
                    ∃ v', ⌜v = SOMEV v'⌝ ∗ Ψ v' }}) -∗
-  is_conn_state cs n -∗ φ -∗ WP Connection.recv N c (repr cs) f {{ Ψ }}.
+  cs_ts cs ↦ #n -∗ φ -∗ WP Connection.recv N c (repr cs) f {{ Ψ }}.
 Proof.
-iIntros "#chan #pred #post conn inv".
+iIntros "#chan #pred #conn #post ts inv".
+iPoseProof "conn" as "(#minted_kS & #p_kS & #sess)".
 wp_lam; wp_pures.
-wp_bind (Connection.session_key _).
-iApply (wp_connection_session_key with "conn").
-iIntros "!> (conn & #minted_kS & #p_kS & #sess)".
-wp_pures. iCombine "conn inv" as "I". iRevert "I".
+wp_apply wp_connection_session_key => //. iIntros "_".
+wp_pures. iCombine "ts inv" as "I". iRevert "I".
 iApply wp_do_until.
-iIntros "!> (conn & inv)".
+iIntros "!> (ts & inv)".
 wp_pure _ credit:"c".
-wp_pures. wp_bind (recv _). iApply wp_recv => //.
+wp_pures. wp_apply wp_recv => //.
 iIntros "%m #p_m". wp_pures. wp_sdec m; wp_pures; last by iLeft; iFrame.
 iAssert (▷ □ (public m ∗ (failure (si_init cs) (si_resp cs) ∨ Φ cs m)))%I
   as "{p_m} p_m".
@@ -355,15 +352,15 @@ iAssert (▷ □ (public m ∗ (failure (si_init cs) (si_resp cs) ∨ Φ cs m)))
     iDestruct "sess" as "[fail|#sess]"; first by eauto.
     rewrite (session_agree e_kS). by eauto. }
 iMod (lc_fupd_elim_later with "c p_m") as "{p_m} [#p_m #inv_m]".
-by iApply ("post" with "conn inv").
+by iApply ("post" with "ts inv").
 Qed.
 
 Lemma wp_connection_close (c : val) cs n :
-  {{{ is_conn_state cs n }}}
+  {{{ cs_ts cs ↦ #n }}}
     Connection.close c (repr cs)
   {{{ RET #(); True }}}.
 Proof.
-iIntros "%Φ (conn & _) post".
+iIntros "%Φ ts post".
 wp_lam; wp_pures.
 wp_free.
 by iApply "post".
